thread-local invariants are now called non-atomic, and they handle their masks differently

theories/lifetime/tl_borrow.v
@@ -1,51 +1,51 @@
 From lrust.lifetime Require Export derived.
-From iris.base_logic.lib Require Export thread_local.
+From iris.base_logic.lib Require Export na_invariants.
 From iris.proofmode Require Import tactics.
 
-Definition tl_bor `{invG Σ, lftG Σ, thread_localG Σ}
+Definition na_bor `{invG Σ, lftG Σ, na_invG Σ}
            (κ : lft) (tid : thread_id) (N : namespace) (P : iProp Σ) :=
-  (∃ i, &{κ,i}P ∗ tl_inv tid N (idx_bor_own 1 i))%I.
+  (∃ i, &{κ,i}P ∗ na_inv tid N (idx_bor_own 1 i))%I.
 
-Notation "&tl{ κ , tid , N } P" := (tl_bor κ tid N P)
-  (format "&tl{ κ , tid , N } P", at level 20, right associativity) : uPred_scope.
+Notation "&na{ κ , tid , N } P" := (na_bor κ tid N P)
+  (format "&na{ κ , tid , N } P", at level 20, right associativity) : uPred_scope.
 
-Section tl_bor.
-  Context `{invG Σ, lftG Σ, thread_localG Σ}
+Section na_bor.
+  Context `{invG Σ, lftG Σ, na_invG Σ}
           (tid : thread_id) (N : namespace) (P : iProp Σ).
 
-  Global Instance tl_bor_persistent κ : PersistentP (&tl{κ,tid,N} P) := _.
-  Global Instance tl_bor_proper κ :
-    Proper ((⊣⊢) ==> (⊣⊢)) (tl_bor κ tid N).
+  Global Instance na_bor_persistent κ : PersistentP (&na{κ,tid,N} P) := _.
+  Global Instance na_bor_proper κ :
+    Proper ((⊣⊢) ==> (⊣⊢)) (na_bor κ tid N).
   Proof.
     intros P1 P2 EQ. apply uPred.exist_proper. intros i. by rewrite EQ.
   Qed.
 
-  Lemma bor_tl κ E : ↑lftN ⊆ E → &{κ}P ={E}=∗ &tl{κ,tid,N}P.
+  Lemma bor_na κ E : ↑lftN ⊆ E → &{κ}P ={E}=∗ &na{κ,tid,N}P.
   Proof.
     iIntros (?) "HP". rewrite bor_unfold_idx. iDestruct "HP" as (i) "[#? Hown]".
-    iExists i. iFrame "#". iApply (tl_inv_alloc tid E N with "[Hown]"). auto.
+    iExists i. iFrame "#". iApply (na_inv_alloc tid E N with "[Hown]"). auto.
   Qed.
 
-  Lemma tl_bor_acc q κ E F :
-    ↑lftN ⊆ E → ↑tlN ⊆ E → ↑N ⊆ F →
-    lft_ctx -∗ &tl{κ,tid,N}P -∗ q.[κ] -∗ tl_own tid F ={E}=∗
-            ▷P ∗ tl_own tid (F ∖ ↑N) ∗
-            (▷P -∗ tl_own tid (F ∖ ↑N) ={E}=∗ q.[κ] ∗ tl_own tid F).
+  Lemma na_bor_acc q κ E :
+    ↑lftN ⊆ E → ↑N ⊆ E →
+    lft_ctx -∗ &na{κ,tid,N}P -∗ q.[κ] -∗ na_own tid E ={E}=∗
+            ▷P ∗ na_own tid (E ∖ ↑N) ∗
+            (▷P -∗ na_own tid (E ∖ ↑N) ={E}=∗ q.[κ] ∗ na_own tid E).
   Proof.
-    iIntros (???) "#LFT#HP Hκ Htlown".
+    iIntros (??) "#LFT#HP Hκ Hnaown".
     iDestruct "HP" as (i) "(#Hpers&#Hinv)".
-    iMod (tl_inv_open with "Hinv Htlown") as "(>Hown&Htlown&Hclose)"; try done.
+    iMod (na_inv_open with "Hinv Hnaown") as "(>Hown&Hnaown&Hclose)"; try done.
     iMod (idx_bor_acc with "LFT Hpers Hown Hκ") as "[HP Hclose']". done.
-    iIntros "{$HP $Htlown}!>HP Htlown".
+    iIntros "{$HP $Hnaown}!>HP Hnaown".
     iMod ("Hclose'" with "HP") as "[Hown $]". iApply "Hclose". by iFrame.
   Qed.
 
-  Lemma tl_bor_shorten κ κ': κ ⊑ κ' -∗ &tl{κ',tid,N}P -∗ &tl{κ,tid,N}P.
+  Lemma na_bor_shorten κ κ': κ ⊑ κ' -∗ &na{κ',tid,N}P -∗ &na{κ,tid,N}P.
   Proof.
     iIntros "Hκκ' H". iDestruct "H" as (i) "[??]". iExists i. iFrame.
     iApply (idx_bor_shorten with "Hκκ' H").
   Qed.
 
-End tl_bor.
+End na_bor.
 
-Typeclasses Opaque tl_bor.
+Typeclasses Opaque na_bor.
